Add and prove [auto_node_in_list_is_included]

ind/DoublyLinkedListIface.fst
@@ -423,3 +423,16 @@ let auto_node_val_unchanged_staying_unchanged h0 h1 n =()
 /// manually. If you do, it is (likely) a bug wrt the patterns, and
 /// you should ask someone who knows about how this library works to
 /// look at things.
+
+let auto_node_in_list_is_included h0 n d =
+  let rec aux (n:node 'a) (nl:list (node 'a)) :
+    Lemma
+      (requires (n `L.memP` nl))
+      (ensures (DLL.nodelist_fp0 nl `B.loc_includes` fp_node n)) =
+    match nl with
+    | [_] -> ()
+    | n' :: ns ->
+      FStar.Classical.or_elim #_ #_ #(fun () -> DLL.nodelist_fp0 nl `B.loc_includes` fp_node n)
+        (fun (_:unit{n == n'}) -> ())
+        (fun (_:unit{n =!= n'}) -> aux n ns) in
+  aux n (as_list h0 d)
